updated to latest version of lean

examples.lean
@@ -5,10 +5,10 @@ import data.list.basic
 import util.logic
 import util.control.applicative
 import util.control.monad.non_termination
-import ..separation.heap
-import ..separation.program
-import ..separation.specification
-import ..separation.tactics
+import separation.heap
+import separation.program
+import separation.specification
+import separation.tactics
 
 universes u v w w'
 
@@ -32,7 +32,7 @@ lemma swap_ptr_spec (p q : pointer) (v₀ v₁ : word)
                      , post := λ _, p ↦ v₁ :*: q ↦ v₀ } :=
 begin
   unfold swap_ptr,
-  bind_step t with h,
+  bind_step with t h,
   bind_step,
   bind_step,
   bind_step,
@@ -81,7 +81,7 @@ begin
     extract_context h,
     rw embed_s_and_self,
     rw [map_list_def],
-    rw if_pos h,
+    simp [h],
     apply return.spec' },
   case cons x xs
   { unfold map is_list,
@@ -89,8 +89,8 @@ begin
     rw [map_list_def],
     rw if_neg Hp_nz, simp,
     bind_step,
-    bind_step with h,
-    unfold replace nth_le at *, subst x_1,
+    bind_step with _ h,
+    unfold replace nth_le at *,
     last_step (ih_1 nx.to_ptr), }
 end
 
@@ -131,8 +131,7 @@ begin
   { simp [is_list],
     s_intros nx h,
     rw [list_reverse_aux_def,if_neg h],
-    bind_step p' with h',
-    subst p',
+    bind_step with p' h',
     bind_step, unfold replace const,
     last_step (ih_1 (x :: ys)), }
 end
@@ -164,19 +163,20 @@ def list_reverse_dup_aux : pointer → pointer → program pointer :=
 fix2 (λ list_reverse_dup_aux p q,
 if p = 0 then return q
 else do
-  x  ← read_nth p 0 2 dec_trivial,
+  x  ← read_nth p 0 2,
   q' ← alloc [x,⟨ q ⟩],
-  p' ← read_nth p 1 2 dec_trivial,
+  p' ← read_nth p 1 2,
   list_reverse_dup_aux p'.to_ptr q')
 
 lemma list_reverse_dup_aux_def (p q : pointer)
 : list_reverse_dup_aux p q =
   if p = 0 then return q
   else do
-    x  ← read_nth p 0 2 dec_trivial,
-    q' ← alloc [x,⟨ q ⟩],
-    p' ← read_nth p 1 2 dec_trivial,
-    list_reverse_dup_aux p'.to_ptr q' := sorry
+    x  ← read_nth p 0 2,
+    new ← alloc [x,⟨ q ⟩],
+    next ← read_nth p 1 2,
+    list_reverse_dup_aux next.to_ptr new :=
+sorry
 
 def segment : pointer → pointer → list word → hprop
  | p q [] := [| p = q |]
@@ -186,6 +186,7 @@ lemma segment_nil (p : pointer) (xs : list word)
 : segment p 0 xs = is_list p xs :=
 sorry
 
+@[ptr_abstraction]
 lemma segment_append (p q : pointer) (xs ys : list word)
 : segment p q (xs++ys) = ∃∃ r, segment p q xs :*: segment q r ys :=
 sorry
@@ -199,12 +200,12 @@ lemma list_reverse_dup_aux_spec (p q r : pointer) (xs ys zs : list word)
       { pre := segment p q xs :*: is_list q ys :*: is_list r zs,
         post := λ q, is_list p (xs ++ ys) :*: is_list q (list.reverse ys ++ zs) } :=
 begin
-  revert xs q zs r,
-  induction ys ; intros xs q zs r,
+  revert xs zs q r,
+  induction ys ; intros xs zs q r,
   case nil
   { unfold is_list,
     extract_context h,
-    rw [list_reverse_dup_aux_def,if_pos h],
+    rw [list_reverse_dup_aux_def],
     subst q, simp [segment_nil],
     apply postcondition _ (return.spec _ _),
     { intros, dsimp [list.reverse_nil], ac_refl } },
@@ -213,22 +214,26 @@ begin
     extract_context h,
     s_exists nx,
     rw [list_reverse_dup_aux_def,if_neg h],
-    bind_step ry with h₀,
-    bind_step q' with h₁,
-    bind_step p' with h₂,
-    subst ry, subst p',
+    bind_step with x  h₀,
+    bind_step with new h₁,
+    bind_step with next h,
+    repeat { rw [← s_and_assoc] },
+    have HH := (ih_1 (xs ++ [x]) (x :: zs) next.to_ptr new),
+    -- last_step (ih_1 (xs ++ [y]) (y :: zs)),
     -- apply s_exists_elim_pre nx,
     -- apply s_exists_replace_pre word.to_word word.to_ptr,
     -- { intro, cases x, refl },
-    have HH := (ih_1 (xs ++ [y]) _ (y :: zs) _),
+    -- have HH := (ih_1 (xs ++ [y]) (y :: zs) _),
 
     apply framing_spec' _ HH,
     { simp [segment_append,is_list],
       simp [s_exists_s_and_distr,s_and_s_exists_distr],
-      -- apply s_exists_intro,
-      -- apply s_exists_intro,
+      apply s_exists_intro (word.to_word r),
+      apply s_exists_intro,
+      simp [embed_eq_emp h₁],
+      -- ac_match',
       -- apply s_imp_of_eq, simp [embed_eq_emp h₂,s_and_assoc],
-      admit },
+      admit, admit },
     { intro, simp, rw [s_and_emp] }, },
 end
 
@@ -250,6 +255,7 @@ inductive tree (α : Type u)
   | leaf {} : tree
   | node : tree → α → tree → tree
 
+@[ptr_abstraction]
 def is_tree : pointer → tree word → hprop
   | p tree.leaf := [| p = 0 |]
   | p (tree.node l x r) := ∃∃ lp rp : word,
@@ -259,12 +265,48 @@ def is_tree : pointer → tree word → hprop
           is_tree rp.to_ptr r
 
 def free_tree : pointer → program unit :=
+fix λ free_tree p, do
+if p = 0 then return ()
+else do
+  l ← read_nth p 0 3,
+  r ← read_nth p 2 3,
+  free p 3,
+  free_tree l.to_ptr,
+  free_tree r.to_ptr
+
+lemma free_tree_def (p : pointer)
+: free_tree p =
+  if p = 0 then return ()
+  else do
+    l ← read_nth p 0 3,
+    r ← read_nth p 2 3,
+    free p 3,
+    free_tree l.to_ptr,
+    free_tree r.to_ptr :=
 sorry
 
 lemma free_tree_spec (p : pointer) (t : tree word)
 : sat (free_tree p) { pre := is_tree p t
                     , post := λ _, emp } :=
-sorry
+begin
+  revert p,
+  induction t ; intro p,
+  case tree.leaf
+  { unfold is_tree,
+    rw free_tree_def,
+    s_intros h,
+    simp [h],
+    apply return.spec', },
+  case tree.node l x r
+  { unfold is_tree,
+    s_intros lp rp h,
+    rw [free_tree_def,if_neg h],
+    bind_step with l hl,
+    bind_step with r hr,
+    bind_step,
+    bind_step ih_1,
+    last_step ih_2 }
+end
 
 end examples
 
